Migrate VMPath to ValidPos

correctness/RegexCorrectness/VM/Path/CharStep.lean
@@ -2,66 +2,70 @@ import RegexCorrectness.NFA.Semantics.Path
 
 set_option autoImplicit false
 
-open String (Iterator)
+open String (ValidPos)
 
 namespace Regex.NFA
 
-def CharStep (nfa : NFA) (it : Iterator) (i j : Fin nfa.nodes.size) : Prop :=
-  nfa.Step 0 i it j it.next .none
+def CharStep {s : String} (nfa : NFA) (pos : ValidPos s) (i j : Fin nfa.nodes.size) : Prop :=
+  ∃ ne : pos ≠ s.endValidPos, nfa.Step 0 i pos j (pos.next ne) .none
 
 namespace CharStep
 
-variable {nfa : NFA} {it : Iterator} {i j : Fin nfa.nodes.size}
+variable {s : String} {nfa : NFA} {pos : ValidPos s} {i j : Fin nfa.nodes.size}
 
-@[simp]
+@[grind →]
+theorem ne (step : nfa.CharStep pos i j) : pos ≠ s.endValidPos := by
+  grind [CharStep]
+
+@[grind →]
+theorem step (step : nfa.CharStep pos i j) :
+  nfa.Step 0 i pos j (pos.next step.ne) .none := by
+  grind [CharStep]
+
+@[simp, grind =]
 theorem done (hn : nfa[i] = .done) :
-  nfa.CharStep it i j ↔ False := by
-  apply Step.iff_done hn
+  nfa.CharStep pos i j ↔ False := by
+  simp [CharStep, Step.iff_done hn]
 
-@[simp]
+@[simp, grind =]
 theorem fail (hn : nfa[i] = .fail) :
-  nfa.CharStep it i j ↔ False := by
-  apply Step.iff_fail hn
+  nfa.CharStep pos i j ↔ False := by
+  simp [CharStep, Step.iff_fail hn]
 
-@[simp]
+@[simp, grind =>]
 theorem epsilon {next} (hn : nfa[i] = .epsilon next) :
-  nfa.CharStep it i j ↔ False := by
-  simp [CharStep, Step.iff_epsilon hn]
+  nfa.CharStep pos i j ↔ False := by
+  simp [CharStep, Step.iff_epsilon hn, pos.ne_next.symm]
 
-@[simp]
+@[simp, grind =>]
 theorem anchor {anchor next} (hn : nfa[i] = .anchor anchor next) :
-  nfa.CharStep it i j ↔ False := by
-  simp [CharStep, Step.iff_anchor hn]
+  nfa.CharStep pos i j ↔ False := by
+  simp [CharStep, Step.iff_anchor hn, pos.ne_next.symm]
 
-@[simp]
+@[simp, grind =>]
 theorem split {next₁ next₂} (hn : nfa[i] = .split next₁ next₂) :
-  nfa.CharStep it i j ↔ False := by
-  simp [CharStep, Step.iff_split hn]
+  nfa.CharStep pos i j ↔ False := by
+  simp [CharStep, Step.iff_split hn, pos.ne_next.symm]
 
-@[simp]
+@[simp, grind =>]
 theorem save {offset next} (hn : nfa[i] = .save offset next) :
-  nfa.CharStep it i j ↔ False := by
+  nfa.CharStep pos i j ↔ False := by
   simp [CharStep, Step.iff_save hn]
 
-@[simp]
+@[simp, grind =>]
 theorem char {c next} (hn : nfa[i] = .char c next) :
-  nfa.CharStep it i j ↔ ∃ l r, j = next ∧ it.ValidFor l (c :: r) := by
+  nfa.CharStep pos i j ↔ ∃ ne : pos ≠ s.endValidPos, j = next ∧ pos.get ne = c := by
   simp [CharStep, Step.iff_char hn]
 
-@[simp]
+@[simp, grind =>]
 theorem sparse {cs next} (hn : nfa[i] = .sparse cs next) :
-  nfa.CharStep it i j ↔ ∃ l c r, j = next ∧ it.ValidFor l (c :: r) ∧ c ∈ cs := by
+  nfa.CharStep pos i j ↔ ∃ ne : pos ≠ s.endValidPos, j = next ∧ pos.get ne ∈ cs := by
   simp [CharStep, Step.iff_sparse hn]
 
-theorem char_or_sparse (step : nfa.CharStep it i j) :
+@[grind .]
+theorem char_or_sparse (step : nfa.CharStep pos i j) :
   (∃ c next, nfa[i] = .char c next) ∨ (∃ cs next, nfa[i] = .sparse cs next) := by
-  match hn : nfa[i] with
-  | .char c next => simp
-  | .sparse cs next => simp
-  | .done | .fail | .epsilon _ => simp_all
-  | .anchor _ _ => simp [anchor hn] at step
-  | .split _ _ => simp [split hn] at step
-  | .save _ _ => simp [save hn] at step
+  grind [CharStep]
 
 end CharStep
 
