correctness/RegexCorrectness/VM/Path/VMPath.lean
@@ -7,125 +7,103 @@ set_option autoImplicit false
 
 open Regex.Data (SparseSet)
 open Regex (NFA)
-open String (Iterator)
-open String.Pos (Raw)
+open String (ValidPos)
 
 namespace Regex.NFA
 
-theorem Step.εStep_or_charStep {nfa : NFA} {it it' i j update} (wf : nfa.WellFormed) (step : nfa.Step 0 i it j it' update) :
-  (nfa.εStep' it ⟨i, step.lt⟩ ⟨j, step.lt_right wf⟩ update ∧ it' = it) ∨
-  (nfa.CharStep it ⟨i, step.lt⟩ ⟨j, step.lt_right wf⟩ ∧ it' = it.next ∧ update = .none) := by
-  cases step with
-  | epsilon ge lt v eq => exact .inl ⟨Step.epsilon ge lt v eq, rfl⟩
-  | anchor ge lt eq v htest => exact .inl ⟨Step.anchor ge lt eq v htest, rfl⟩
-  | splitLeft ge lt eq v => exact .inl ⟨Step.splitLeft ge lt eq v, rfl⟩
-  | splitRight ge lt eq v => exact .inl ⟨Step.splitRight ge lt eq v, rfl⟩
-  | save ge lt eq v => exact .inl ⟨Step.save ge lt eq v, rfl⟩
-  | char ge lt eq vf => exact .inr ⟨Step.char ge lt eq vf, rfl, rfl⟩
-  | sparse ge lt eq mem vf => exact .inr ⟨Step.sparse ge lt eq mem vf, rfl, rfl⟩
+variable {s : String} {nfa : NFA} {wf : nfa.WellFormed} {pos₀ pos pos' : ValidPos s} {i j : Fin nfa.nodes.size} {update : Option (Nat × ValidPos s)}
 
-inductive VMPath (nfa : NFA) (wf : nfa.WellFormed) (it₀ : Iterator) : Iterator → Fin nfa.nodes.size → List (Nat × Raw) → Prop where
-  | init {it i update} (eqs : it.toString = it₀.toString) (le : it₀.pos ≤ it.pos) (cls : nfa.εClosure' it ⟨nfa.start, wf.start_lt⟩ i update) :
-    VMPath nfa wf it₀ it i update
-  | more {i j k it it' update₁ update₂ update₃} (prev : VMPath nfa wf it₀ it i update₁) (step : nfa.CharStep it i j) (cls : nfa.εClosure' it.next j k update₂)
-    (hupdate : update₃ = update₁ ++ update₂) (eqit : it' = it.next) :
-    VMPath nfa wf it₀ it' k update₃
+@[grind →]
+theorem Step.εStep_or_charStep {i j : Nat} (wf : nfa.WellFormed) (step : nfa.Step 0 i pos j pos' update) :
+  (nfa.εStep' pos ⟨i, step.lt⟩ ⟨j, step.lt_right wf⟩ update ∧ pos' = pos) ∨
+  (nfa.CharStep pos ⟨i, step.lt⟩ ⟨j, step.lt_right wf⟩ ∧ update = .none ∧ ∃ ne, pos' = pos.next ne) := by
+  grind
+
+inductive VMPath (nfa : NFA) (wf : nfa.WellFormed) (pos₀ : ValidPos s) : ValidPos s → Fin nfa.nodes.size → List (Nat × ValidPos s) → Prop where
+  | init {pos i update} (le : pos₀ ≤ pos) (cls : nfa.εClosure' pos ⟨nfa.start, wf.start_lt⟩ i update) :
+    VMPath nfa wf pos₀ pos i update
+  | more {i j k pos pos' update₁ update₂ update₃} (prev : VMPath nfa wf pos₀ pos i update₁) (step : nfa.CharStep pos i j) (cls : nfa.εClosure' (pos.next step.ne) j k update₂)
+    (hupdate : update₃ = update₁ ++ update₂) (hpos : pos' = pos.next step.ne) :
+    VMPath nfa wf pos₀ pos' k update₃
 
 namespace VMPath
 
-theorem more_εStep {nfa : NFA} {wf it₀ it i j update₁ update₂}
-  (prev : nfa.VMPath wf it₀ it i update₁) (step : nfa.εStep' it i j update₂) :
-  nfa.VMPath wf it₀ it j (update₁ ++ List.ofOption update₂) := by
+theorem more_εStep {update₁ update₂}
+  (prev : nfa.VMPath wf pos₀ pos i update₁) (step : nfa.εStep' pos i j update₂) :
+  nfa.VMPath wf pos₀ pos j (update₁ ++ List.ofOption update₂) := by
   cases prev with
-  | init eqs le cls => exact .init eqs le (cls.snoc step)
+  | init le cls => exact .init le (cls.snoc step)
   | more prev step' cls hupdate eqit => exact .more prev step' (cls.snoc (eqit ▸ step)) (by simp [hupdate]) eqit
 
-theorem more_charStep {nfa : NFA} {wf it₀ it i j update}
-  (prev : nfa.VMPath wf it₀ it i update) (step : nfa.CharStep it i j) :
-  nfa.VMPath wf it₀ it.next j update := by
+theorem more_charStep {update} (prev : nfa.VMPath wf pos₀ pos i update) (step : nfa.CharStep pos i j) :
+  nfa.VMPath wf pos₀ (pos.next step.ne) j update := by
   cases prev with
-  | init eqs le cls => exact .more (.init eqs le cls) step (.base step.validR) (by simp) rfl
-  | more prev step' cls hupdate eqit => exact .more (.more prev step' cls hupdate eqit) step (.base step.validR) (by simp) rfl
+  | init le cls => exact .more (.init le cls) step .base (by simp) rfl
+  | more prev step' cls hupdate eqit => exact .more (.more prev step' cls hupdate eqit) step .base (by simp) rfl
 
-theorem more_step {nfa : NFA} {wf it₀ it it' i j update₁ update₂}
-  (prev : nfa.VMPath wf it₀ it i update₁) (step : nfa.Step 0 i it j it' update₂) :
-  nfa.VMPath wf it₀ it' ⟨j, step.lt_right wf⟩ (update₁ ++ List.ofOption update₂) := by
+theorem more_step {j : Nat} {update₁ update₂}
+  (prev : nfa.VMPath wf pos₀ pos i update₁) (step : nfa.Step 0 i pos j pos' update₂) :
+  nfa.VMPath wf pos₀ pos' ⟨j, step.lt_right wf⟩ (update₁ ++ List.ofOption update₂) := by
   match step.εStep_or_charStep wf with
-  | .inl ⟨step, eqit⟩ => exact eqit ▸ prev.more_εStep step
-  | .inr ⟨step, eqit, equpdate⟩ => simpa [eqit, equpdate] using prev.more_charStep step
+  | .inl ⟨step, hpos⟩ => exact hpos ▸ prev.more_εStep step
+  | .inr ⟨step, hupdate, ne, hpos⟩ => simpa [hupdate, hpos] using prev.more_charStep step
 
-theorem valid {nfa : NFA} {wf it₀ it i update} (path : nfa.VMPath wf it₀ it i update) : it.Valid := by
+theorem le {update} (path : nfa.VMPath wf pos₀ pos i update) :
+  pos₀ ≤ pos := by
+  induction path with
+  | init le _ => exact le
+  | @more i j k pos' pos _ _ _ _ _ _ _ hpos ih =>
+    rw [hpos]
+    exact Nat.le_trans ih (Nat.le_of_lt pos'.lt_next)
+
+theorem εClosure_of_eq_it {update} (path : nfa.VMPath wf pos pos i update) :
+  nfa.εClosure' pos ⟨nfa.start, wf.start_lt⟩ i update := by
   cases path with
-  | init _ _ cls => exact cls.valid
-  | more _ _ cls _ eqit => exact eqit ▸ cls.valid
+  | init _ cls => exact cls
+  | @more i j k pos' pos _ _ _ prev step _ _ hpos =>
+    have le := prev.le
+    rw [hpos] at le
+    exact (Nat.not_lt_of_ge le pos'.lt_next).elim
 
-theorem toString {nfa : NFA} {wf it₀ it i update} (path : nfa.VMPath wf it₀ it i update) :
-  it.toString = it₀.toString := by
+theorem eq_or_nfaPath {update} (path : nfa.VMPath wf pos₀ pos i update) :
+  (i.val = nfa.start ∧ update = [] ∧ pos₀ ≤ pos) ∨
+  ∃ poss, pos₀ ≤ poss ∧ nfa.Path 0 nfa.start poss i pos update := by
   induction path with
-  | init eqs => exact eqs
-  | more _ _ _ _ eqit ih =>
-    rw [eqit, Iterator.next_toString, ih]
-
-theorem le_pos {nfa : NFA} {wf it₀ it i update} (path : nfa.VMPath wf it₀ it i update) :
-  it₀.pos ≤ it.pos := by
-  induction path with
-  | init _ le _ => exact le
-  | @more i j k it' it _ _ _ _ _ _ _ eqit ih =>
-    rw [eqit]
-    exact Nat.le_trans ih (Nat.le_of_lt it'.lt_next)
-
-theorem εClosure_of_eq_it {nfa : NFA} {wf it i update} (path : nfa.VMPath wf it it i update) :
-  nfa.εClosure' it ⟨nfa.start, wf.start_lt⟩ i update := by
-  cases path with
-  | init _ _ cls => exact cls
-  | @more i j k it' it _ _ _ prev step _ _ eqit =>
-    have le := prev.le_pos
-    rw [eqit] at le
-    exact (Nat.not_lt_of_ge le it'.lt_next).elim
-
-theorem eq_or_nfaPath {nfa : NFA} {wf it₀ it i update} (path : nfa.VMPath wf it₀ it i update) :
-  (i.val = nfa.start ∧ update = [] ∧ it.toString = it₀.toString ∧ it₀.pos ≤ it.pos) ∨
-  ∃ its, its.toString = it₀.toString ∧ it₀.pos ≤ its.pos ∧ nfa.Path 0 nfa.start its i it update := by
-  induction path with
-  | @init itp i update eqs le cls =>
-    simp [εClosure'_iff_path nfa wf] at cls
+  | @init pos i update le cls =>
+    simp only [εClosure'_iff_path nfa wf] at cls
     cases cls with
-    | inl h => simp [←h.1, h.2, eqs, le, -Iterator.toString, -Iterator.pos]
-    | inr cls => exact .inr ⟨itp, eqs, le, cls⟩
-  | @more i j k it it' update₁ update₂ update₃ prev step cls equpdate eqit ih =>
-    have path₂ : nfa.Path 0 i it k it.next update₂ := by
-      simp [εClosure'_iff_path nfa wf] at cls
+    | inl h => simp [←h.1, h.2, le]
+    | inr cls => exact .inr ⟨pos, le, cls⟩
+  | @more i j k pos pos' update₁ update₂ update₃ prev step cls hupdate hpos ih =>
+    have path₂ : nfa.Path 0 i pos k (pos.next step.ne) update₂ := by
+      simp only [εClosure'_iff_path nfa wf] at cls
       match cls with
-      | .inl ⟨eqk, equpdate, v⟩ =>
-        rw [←eqk, equpdate]
-        exact .last step
-      | .inr path => exact .more step path
-
+      | .inl ⟨eqk, hupdate⟩ =>
+        rw [←eqk, hupdate]
+        exact .last step.step
+      | .inr path => exact .more step.step path
     match ih with
-    | .inl ⟨eqi, equpdate', eqs, le⟩ =>
-      simp [←eqi]
-      simp [equpdate'] at equpdate
-      exact .inr ⟨it, eqs, le, equpdate ▸ eqit ▸ path₂⟩
-    | .inr ⟨itp, eqs, le, path₁⟩ => exact .inr ⟨itp, eqs, le, equpdate ▸ eqit ▸ path₁.trans path₂⟩
+    | .inl ⟨eqi, hupdate', le⟩ =>
+      simp only [← eqi]
+      simp only [hupdate'] at hupdate
+      exact .inr ⟨pos, le, hupdate ▸ hpos ▸ path₂⟩
+    | .inr ⟨poss, le, path₁⟩ => exact .inr ⟨poss, le, hupdate ▸ hpos ▸ path₁.trans path₂⟩
 
-theorem nfaPath_of_ne {nfa : NFA} {wf it₀ it i update} (path : nfa.VMPath wf it₀ it i update)
-  (ne : i.val ≠ nfa.start):
-  ∃ its, its.toString = it₀.toString ∧ it₀.pos ≤ its.pos ∧ nfa.Path 0 nfa.start its i it update := by
+theorem nfaPath_of_ne {update} (path : nfa.VMPath wf pos₀ pos i update) (ne : i.val ≠ nfa.start) :
+  ∃ poss, pos₀ ≤ poss ∧ nfa.Path 0 nfa.start poss i pos update := by
   simpa [ne] using eq_or_nfaPath path
 
-theorem concat_nfaPath {nfa : NFA} {wf it₀ it it' i j update₁ update₂}
-  (isLt₁ : i < nfa.nodes.size)
-  (path₁ : nfa.VMPath wf it₀ it ⟨i, isLt₁⟩ update₁) (path₂ : nfa.Path 0 i it j it' update₂) :
-  nfa.VMPath wf it₀ it' ⟨j, path₂.lt_right wf⟩ (update₁ ++ update₂) := by
+theorem concat_nfaPath {i j : Nat} {update₁ update₂} (isLt₁ : i < nfa.nodes.size)
+  (path₁ : nfa.VMPath wf pos₀ pos ⟨i, isLt₁⟩ update₁) (path₂ : nfa.Path 0 i pos j pos' update₂) :
+  nfa.VMPath wf pos₀ pos' ⟨j, path₂.lt_right wf⟩ (update₁ ++ update₂) := by
   induction path₂ generalizing update₁ with
-  | @last j it k it' update₂ step => exact path₁.more_step step
-  | @more j it k it' l it'' update₂ update₃ step rest ih => simpa using ih rest.lt (path₁.more_step step)
+  | @last j pos k pos' update₂ step => exact path₁.more_step step
+  | @more j pos k pos' l pos'' update₂ update₃ step rest ih => simpa using ih rest.lt (path₁.more_step step)
 
-theorem of_nfaPath {nfa : NFA} {it₀ it it' i update} (wf : nfa.WellFormed)
-  (eqs : it.toString = it₀.toString) (le : it₀.pos ≤ it.pos)
-  (path : nfa.Path 0 nfa.start it i it' update) :
-  nfa.VMPath wf it₀ it' ⟨i, path.lt_right wf⟩ update := by
-  have path₁ : nfa.VMPath wf it₀ it ⟨nfa.start, wf.start_lt⟩ [] := .init eqs le (.base path.validL)
+theorem of_nfaPath {i : Nat} {update} (wf : nfa.WellFormed)
+  (le : pos₀ ≤ pos) (path : nfa.Path 0 nfa.start pos i pos' update) :
+  nfa.VMPath wf pos₀ pos' ⟨i, path.lt_right wf⟩ update := by
+  have path₁ : nfa.VMPath wf pos₀ pos ⟨nfa.start, wf.start_lt⟩ [] := .init le .base
   exact path₁.concat_nfaPath wf.start_lt path
 
 end VMPath
@@ -134,48 +112,50 @@ end Regex.NFA
 
 namespace Regex.VM
 
+variable {s : String}
+
 /--
 The invariant for the soundness theorem.
 
-All states in `next.state` have a corresponding path from `nfa.start` to the state ending at `it`,
+All states in `next.state` have a corresponding path from `nfa.start` to the state ending at `pos`,
 and their updates are written to `next.updates` when necessary.
 -/
-def SearchState.Inv (nfa : NFA) (wf : nfa.WellFormed) (it₀ it : Iterator) (next : SearchState HistoryStrategy nfa) : Prop :=
+def SearchState.Inv (nfa : NFA) (wf : nfa.WellFormed) (pos₀ pos : ValidPos s) (next : SearchState (HistoryStrategy s) nfa) : Prop :=
   ∀ i ∈ next.states,
     ∃ update,
-      nfa.VMPath wf it₀ it i update ∧
+      nfa.VMPath wf pos₀ pos i update ∧
       (εClosure.writeUpdate nfa[i] → next.updates[i] = update)
 
-theorem SearchState.Inv.of_empty {nfa wf it₀ it} {next : SearchState HistoryStrategy nfa} (h : next.states.isEmpty) :
-  next.Inv nfa wf it₀ it := by
+theorem SearchState.Inv.of_empty {nfa wf pos₀ pos} {next : SearchState (HistoryStrategy s) nfa} (h : next.states.isEmpty) :
+  next.Inv nfa wf pos₀ pos := by
   intro i mem
   exact (SparseSet.not_mem_of_isEmpty h mem).elim
 
 /--
 The invariant for the completeness theorem. The invariant holds only when returning `.none`, since we short-circuit when encountering `.done`.
 
-For all paths ending at `it`, the state must be tracked in `next.states`. We don't care about the updates for the completeness.
+For all paths ending at `pos`, the state must be tracked in `next.states`. We don't care about the updates for the completeness.
 -/
-def SearchState.MemOfPathInv (nfa : NFA) (wf : nfa.WellFormed) (it₀ it : Iterator) (next : SearchState HistoryStrategy nfa) : Prop :=
-  ∀ i update, nfa.VMPath wf it₀ it i update → i ∈ next.states
+def SearchState.MemOfPathInv (nfa : NFA) (wf : nfa.WellFormed) (pos₀ pos : ValidPos s) (next : SearchState (HistoryStrategy s) nfa) : Prop :=
+  ∀ i update, nfa.VMPath wf pos₀ pos i update → i ∈ next.states
 
 /--
 Invariant for the completeness theorem.
 
 The `.done` state is not in `next.states`.
 -/
-def SearchState.NotDoneInv (σ : Strategy) (nfa : NFA) (next : SearchState σ nfa) : Prop :=
+def SearchState.NotDoneInv (σ : Strategy s) (nfa : NFA) (next : SearchState σ nfa) : Prop :=
   ∀ i, i ∈ next.states → nfa[i] ≠ .done
 
-theorem SearchState.NotDoneInv.of_empty {σ nfa} {next : SearchState σ nfa} (h : next.states.isEmpty) :
+theorem SearchState.NotDoneInv.of_empty {σ : Strategy s} {nfa : NFA} {next : SearchState σ nfa} (h : next.states.isEmpty) :
   next.NotDoneInv σ nfa := by
   intro i mem
   exact (SparseSet.not_mem_of_isEmpty h mem).elim
 
 end Regex.VM
 
-theorem Regex.NFA.CharStep.write_update {nfa : NFA} {it i j}
-  (step : nfa.CharStep it i j) : Regex.VM.εClosure.writeUpdate nfa[i] := by
+theorem Regex.NFA.CharStep.write_update {s : String} {nfa : NFA} {pos : ValidPos s} {i j}
+  (step : nfa.CharStep pos i j) : Regex.VM.εClosure.writeUpdate nfa[i] := by
   match step.char_or_sparse with
   | .inl ⟨c, next, eq⟩ => simp [Regex.VM.εClosure.writeUpdate, eq]
   | .inr ⟨cs, next, eq⟩ => simp [Regex.VM.εClosure.writeUpdate, eq]
